Soundness.v
@@ -1,0 +1,112 @@
+From Elo Require Import Array.
+From Elo Require Import Map.
+From Elo Require Import Core.
+
+Inductive well_behaved_locations (m : mem) : tm -> Prop :=
+  | wbl_unit :
+    well_behaved_locations m TM_Unit 
+
+  | wbl_num : forall n,
+    well_behaved_locations m (TM_Num n)
+
+  | wbl_loc : forall T ad,
+    empty |-- (getTM m ad) is T ->
+    well_behaved_locations m (TM_Loc T ad)
+
+  | wbl_new : forall T t,
+    well_behaved_locations m t ->
+    well_behaved_locations m (TM_New T t) 
+
+  | wbl_load : forall t,
+    well_behaved_locations m t ->
+    well_behaved_locations m (TM_Load t) 
+
+  | wbl_asg : forall t1 t2,
+    well_behaved_locations m t1 ->
+    well_behaved_locations m t2 ->
+    well_behaved_locations m (TM_Asg t1 t2) 
+
+  | wbl_id : forall id,
+    well_behaved_locations m (TM_Id id)
+
+  | wbl_fun : forall x Tx t,
+    well_behaved_locations m t ->
+    well_behaved_locations m (TM_Fun x Tx t) 
+
+  | wbl_call : forall t1 t2,
+    well_behaved_locations m t1 ->
+    well_behaved_locations m t2 ->
+    well_behaved_locations m (TM_Call t1 t2) 
+
+  | wbl_seq : forall t1 t2,
+    well_behaved_locations m t1 ->
+    well_behaved_locations m t2 ->
+    well_behaved_locations m (TM_Seq t1 t2) 
+
+  | wbl_spawn : forall t,
+    well_behaved_locations m t ->
+    well_behaved_locations m (TM_Spawn t) 
+  .
+
+Lemma context_weakening : forall Gamma Gamma' t T,
+  Gamma includes Gamma' ->
+  Gamma' |-- t is T ->
+  Gamma  |-- t is T.
+Proof.
+  intros. generalize dependent Gamma.
+  induction_type; intros;
+  eauto using well_typed_term, update_preserves_inclusion.
+Qed.
+
+Lemma context_weakening_empty : forall Gamma t T,
+  empty |-- t is T ->
+  Gamma |-- t is T.
+Proof.
+  intros. eapply (context_weakening _ empty); trivial. discriminate.
+Qed.
+
+Lemma substitution_preservation : forall t tx T Tx Tx' Gamma x,
+  Gamma |-- (TM_Fun x Tx t) is (TY_Fun Tx' T) ->
+  empty |-- tx is Tx' ->
+  Gamma |-- [x := tx] t is T.
+Proof.
+  assert (forall t tx T Tx Gamma x,
+    Gamma[x <== Tx] |-- t is T ->
+    empty |-- tx is Tx ->
+    Gamma |-- [x := tx] t is T
+  ). {
+    unfold subst. intros ?.
+    induction t; intros * Htype ?; 
+    try (destruct String.string_dec);
+    inversion Htype; subst; 
+    eauto using well_typed_term, context_weakening, context_weakening_empty,
+      update_overwrite, update_permutation.
+  }
+  intros * ?. inversion_type. intros. eapply H; eauto.
+Qed.
+
+Definition memprop m m' :=
+  (forall ad T,
+  ad < length m ->
+  empty |-- (getTM m ad) is T ->
+  empty |-- (getTM m' ad) is T).
+
+Theorem preservation : forall m m' t t' eff T,
+  well_behaved_locations m t ->
+  empty |-- t is T ->
+  m / t ==[eff]==> m' / t' ->
+  empty |-- t' is T.
+Proof.
+  intros * Hmem Htype ?. inversion_mstep; generalize dependent t'.
+  remember empty as Gamma.
+  - induction Htype; intros; inversion_step; try (inversion Hmem; subst);
+    eauto using well_typed_term, substitution_preservation.
+  - induction Htype; intros; inversion_step; try (inversion Hmem; subst);
+    eauto using well_typed_term.
+  - induction Htype; intros; inversion_step; try (inversion Hmem; subst);
+    eauto using well_typed_term.
+    + inversion Htype; subst. shelve.
+    + inversion Htype; subst. shelve.
+  - induction Htype; intros; inversion_step; eauto using well_typed_term.
+Qed.
+
